examples/sampler/verif_sampler_ingress_parser.v
@@ -73,6 +73,165 @@ Qed.
 Definition parser_parse_ipv4_fundef :=
   ltac:(get_fd ["SwitchIngressParser"; "parse_ipv4"] ge).
 
+Definition IP_PROTOCOLS_TCP: Z := 6.
+Definition IP_PROTOCOLS_UDP: Z := 17.
+
+Record ipv4_rec := {
+    ipv4_version: Val;
+    ipv4_ihl: Val;
+    ipv4_diffserv: Val;
+    ipv4_total_len: Val;
+    ipv4_identification: Val;
+    ipv4_flags: Val;
+    ipv4_frag_offset: Val;
+    ipv4_ttl: Val;
+    ipv4_protocol: Val;
+    ipv4_hdr_checksum: Val;
+    ipv4_src_addr: Val;
+    ipv4_dst_addr: Val;
+  }.
+
+Definition ipv4_repr_val (ipv4: ipv4_rec): Val :=
+  ValBaseHeader
+    [("version", ipv4_version ipv4);
+     ("ihl", ipv4_ihl ipv4);
+     ("diffserv", ipv4_diffserv ipv4);
+     ("total_len", ipv4_total_len ipv4);
+     ("identification", ipv4_identification ipv4);
+     ("flags", ipv4_flags ipv4);
+     ("frag_offset", ipv4_frag_offset ipv4);
+     ("ttl", ipv4_ttl ipv4);
+     ("protocol", ipv4_protocol ipv4);
+     ("hdr_checksum", ipv4_hdr_checksum ipv4);
+     ("src_addr", ipv4_src_addr ipv4);
+     ("dst_addr", ipv4_dst_addr ipv4)] true.
+
+Definition protocol_extract_cond
+  (ipv4: ipv4_rec) (pin pin': packet_in) (result: Val): Prop :=
+  if Val_eqb (ipv4_protocol ipv4) (P4BitV 8 IP_PROTOCOLS_TCP)
+  then extract tcp_h pin = Some (result, SReturnNull, pin')
+  else if Val_eqb (ipv4_protocol ipv4) (P4BitV 8 IP_PROTOCOLS_UDP)
+       then extract udp_h pin = Some (result, SReturnNull, pin')
+       else result = ValBaseNull /\ pin = pin'.
+
+Definition protocol_extract_result
+  (ipv4: ipv4_rec) (result: Val) (header: Sval): Sval :=
+  if Val_eqb (ipv4_protocol ipv4) (P4BitV 8 IP_PROTOCOLS_TCP)
+  then update "tcp" (eval_val_to_sval result) header
+  else if Val_eqb (ipv4_protocol ipv4) (P4BitV 8 IP_PROTOCOLS_UDP)
+       then update "udp" (eval_val_to_sval result) header
+       else header.
+
+Record header_sample_rec := {
+    header_sample_bridge: Sval;
+    header_sample_sample: Sval;
+    header_sample_ethernet: Sval;
+    header_sample_ipv4: Sval;
+    header_sample_tcp: Sval;
+    header_sample_udp: Sval;
+  }.
+
+Definition hdr (hsample: header_sample_rec) :=
+  ValBaseStruct
+    [("bridge", header_sample_bridge hsample);
+     ("sample", header_sample_sample hsample);
+     ("ethernet", header_sample_ethernet hsample);
+     ("ipv4", header_sample_ipv4 hsample);
+     ("tcp", header_sample_tcp hsample);
+     ("udp", header_sample_udp hsample)].
+
+Definition parser_parse_ipv4_spec: func_spec :=
+  WITH,
+    PATH p
+    MOD (Some [["hdr"]]) [["packet_in"]]
+    WITH (pin: packet_in) hsample ipv4 pin2 result pin3
+         (_: extract ipv4_h pin =
+               Some (ipv4_repr_val ipv4, SReturnNull, pin2))
+         (_: protocol_extract_cond ipv4 pin2 pin3 result),
+      PRE
+        (ARG []
+        (MEM [(["hdr"], (hdr hsample))]
+        (EXT [ExtPred.singleton ["packet_in"] (ObjPin pin)])))
+      POST
+        (ARG_RET [] ValBaseNull
+           (MEM [(["hdr"], protocol_extract_result ipv4 result
+                             (update "ipv4" (eval_val_to_sval (ipv4_repr_val ipv4))
+                                (hdr hsample)))]
+           (EXT [ExtPred.singleton ["packet_in"] (ObjPin pin3)]))).
+
+Lemma force_cast_P4BitV_eq: forall w v,
+    force ValBaseNull (@Ops.eval_cast Info (TypBit w) (P4BitV w v)) = P4BitV w v.
+Proof.
+  intros. unfold P4BitV. simpl. f_equal. rewrite P4Arith.bit_to_lbool_back.
+  unfold P4Arith.BitArith.mod_bound. rewrite Zmod_mod.
+  change (v mod _) with (P4Arith.BitArith.mod_bound w v).
+  rewrite P4Arith.to_lbool_bit_mod. reflexivity.
+Qed.
+
+Lemma abs_ipv_hdr_eq_eq: forall ipv4 hsample w v,
+    abs_eq
+      (get "protocol"
+         (get "ipv4"
+            (update "ipv4" (eval_val_to_sval (ipv4_repr_val ipv4))
+               (hdr hsample))))
+      (build_abs_unary_op (@Ops.eval_cast Info (TypBit w))
+         (eval_val_to_sval (P4BitV w v))) =
+      eval_val_to_sval
+        (force ValBaseNull
+           (Ops.eval_binary_op Eq (ipv4_protocol ipv4) (P4BitV w v))).
+Proof.
+  intros. rewrite get_update_same; auto.
+  unfold build_abs_unary_op. rewrite eval_sval_to_val_eq.
+  rewrite force_cast_P4BitV_eq. unfold ipv4_repr_val. simpl get. unfold abs_eq.
+  unfold build_abs_binary_op. rewrite !eval_sval_to_val_eq. reflexivity.
+Qed.
+
+Lemma is_sval_true_binary_op_eq: forall v1 v2,
+  is_sval_true
+    (eval_val_to_sval (force ValBaseNull (Ops.eval_binary_op Eq v1 v2))) ->
+  Val_eqb v1 v2 = true.
+Proof.
+  intros. unfold Ops.eval_binary_op in H.
+  remember (Ops.eval_binary_op_eq _ _).
+  destruct o eqn:?H; simpl in H; [destruct b|]; [|exfalso; auto..].
+  symmetry in Heqo. apply Ops.eval_binary_op_eq_eq in Heqo.
+  rewrite <- Val_eqb_eq_iff in Heqo. assumption.
+Qed.
+
+Lemma is_sval_true_binary_op_neq: forall v1 v2,
+  is_sval_false
+    (eval_val_to_sval (force ValBaseNull (Ops.eval_binary_op Eq v1 v2))) ->
+  Val_eqb v1 v2 = false.
+Proof.
+  intros. unfold Ops.eval_binary_op in H.
+  remember (Ops.eval_binary_op_eq _ _).
+  destruct o eqn:?H; simpl in H; [destruct b|]. 1, 3: exfalso; assumption.
+  symmetry in Heqo. apply Ops.eval_binary_op_neq_neq in Heqo.
+  rewrite <- Val_eqb_eq_iff in Heqo. apply Bool.not_true_is_false in Heqo.
+  assumption.
+Qed.
+
+Lemma parser_parse_ipv4_body:
+  func_sound ge parser_parse_ipv4_fundef nil parser_parse_ipv4_spec.
+Proof.
+  start_function.
+  step_call (@packet_in_extract_body Info); [ entailer | apply H |].
+  step_if; change (ValBaseBit _) with (P4BitV 8 IP_PROTOCOLS_TCP) in H1;
+    rewrite abs_ipv_hdr_eq_eq in H1.
+  - apply is_sval_true_binary_op_eq in H1. red in H0. rewrite H1 in H0.
+    unfold protocol_extract_result. rewrite !H1.
+    step_call parser_parse_tcp_body. 2: apply H0. entailer.
+  - apply is_sval_true_binary_op_neq in H1. red in H0. rewrite H1 in H0.
+    unfold protocol_extract_result. rewrite !H1.
+    step_if; change (ValBaseBit _) with (P4BitV 8 IP_PROTOCOLS_UDP) in H2;
+      rewrite abs_ipv_hdr_eq_eq in H2.
+    + apply is_sval_true_binary_op_eq in H2. rewrite H2 in H0.
+      rewrite !H2. step_call parser_parse_udp_body. 2: apply H0. entailer.
+    + apply is_sval_true_binary_op_neq in H2. rewrite H2 in H0.
+      destruct H0. subst. rewrite !H2.
+      step_call (@parser_accept_body Info). entailer.
+Qed.
+
 Definition parser_parse_ethernet_fundef :=
   ltac:(get_fd ["SwitchIngressParser"; "parse_ethernet"] ge).
 
